src/lib/DY.Lib.fst
@@ -10,6 +10,12 @@ include DY.Lib.Comparse.Parsers
 /// The split function methodology
 include DY.Lib.SplitFunction
 
+/// Split function methodology for cryptographic invariants
+include DY.Lib.Crypto.AEAD.Split
+include DY.Lib.Crypto.KdfExpand.Split
+include DY.Lib.Crypto.PkEncryption.Split
+include DY.Lib.Crypto.Signature.Split
+
 /// User-friendly event API
 include DY.Lib.Event.Typed
 
