src/lib/crypto/DY.Lib.Crypto.PkEncryption.Split.fst
@@ -1,0 +1,59 @@
+module DY.Lib.Crypto.PkEncryption.Split
+
+open Comparse // for_allP, for_allP_eq
+open DY.Core
+open DY.Lib.Crypto.SplitPredicate
+
+let split_pkenc_predicate_params (cusages:crypto_usages): split_crypto_predicate_parameters = {
+  key_t = pk:bytes{PkKey? (get_sk_usage pk)};
+  data_t = bytes;
+  get_usage = (fun pk ->
+    let PkKey tag _ = get_sk_usage pk in
+    tag
+  );
+
+  local_pred_t = pkenc_crypto_predicate cusages;
+  global_pred_t = tr:trace -> pk:bytes{PkKey? (get_sk_usage pk)} -> msg:bytes -> prop;
+
+  apply_local_pred = (fun pred (tr, pk, msg) ->
+    pred.pred tr pk msg
+  );
+  apply_global_pred = (fun pred (tr, pk, msg) ->
+    pred tr pk msg
+  );
+  mk_global_pred = (fun pred tr pk msg ->
+    pred (tr, pk, msg)
+  );
+
+  apply_mk_global_pred = (fun bare x -> ());
+  apply_local_pred_later = (fun lpred tr1 tr2 pk msg ->
+    lpred.pred_later tr1 tr2 pk msg
+  );
+}
+
+val has_pkenc_predicate: cinvs:crypto_invariants -> (string & pkenc_crypto_predicate cinvs.usages) -> prop
+let has_pkenc_predicate cinvs (tag, pred) =
+  has_local_crypto_predicate (split_pkenc_predicate_params cinvs.usages) pkenc_pred.pred (tag, pred)
+
+(*** Global pkenc predicate builder ***)
+
+val mk_pkenc_predicate:
+  {|cusgs:crypto_usages|} ->
+  list (string & pkenc_crypto_predicate cusgs) ->
+  pkenc_crypto_predicate cusgs
+let mk_pkenc_predicate #cusgs l = {
+  pred = mk_global_crypto_predicate (split_pkenc_predicate_params cusgs) l;
+  pred_later = mk_global_crypto_predicate_later (split_pkenc_predicate_params cusgs) l;
+}
+
+val mk_pkenc_predicate_correct:
+  cinvs:crypto_invariants -> tagged_local_preds:list (string & pkenc_crypto_predicate cinvs.usages) ->
+  Lemma
+  (requires
+    pkenc_pred == mk_pkenc_predicate tagged_local_preds /\
+    List.Tot.no_repeats_p (List.Tot.map fst tagged_local_preds)
+  )
+  (ensures for_allP (has_pkenc_predicate cinvs) tagged_local_preds)
+let mk_pkenc_predicate_correct cinvs tagged_local_preds =
+  for_allP_eq (has_pkenc_predicate cinvs) tagged_local_preds;
+  FStar.Classical.forall_intro_2 (FStar.Classical.move_requires_2 (mk_global_crypto_predicate_correct (split_pkenc_predicate_params cinvs.usages) tagged_local_preds))
